Otway-Rees: proved session_st_inv_later

otway-rees/OYRS.Sessions.fst
@@ -154,4 +154,23 @@ let parse_serialize_session_st_lemma i p si vi st =
   | InitiatorRecvedMsg4 srv b k_ab ->
     LC.can_flow_transitive i (LC.get_label MSG.oyrs_key_usages k_ab) (readers [P p]) (readers [V p si vi])
   | _ -> ()
+
+let valid_session_later i j p si vi st =
+  LC.can_flow_later i j (readers [P p]) (readers [P p]);
+  match st with
+  | AuthServerSession pri k_pri_srv ->
+    LC.is_valid_later MSG.oyrs_global_usage i j k_pri_srv
+  | ResponderSentMsg2 srv k_bs a c n_b ->
+    LC.is_valid_later MSG.oyrs_global_usage i j c
+  | AuthServerSentMsg3 a b c n_a n_b k_ab ->
+    LC.is_valid_later MSG.oyrs_global_usage i j c;
+    LC.is_valid_later MSG.oyrs_global_usage i j n_a;
+    LC.is_valid_later MSG.oyrs_global_usage i j n_b
+  | ResponderSentMsg4 srv a k_ab ->
+    LC.is_valid_later MSG.oyrs_global_usage i j k_ab
+  | InitiatorRecvedMsg4 srv b k_ab ->
+    LC.is_valid_later MSG.oyrs_global_usage i j k_ab
+  | _ -> (
+    assert(forall (b:bytes) (l:label). is_labeled i b l /\ later_than j i ==> is_labeled j b l)
+  )
 #pop-options
